Clean up SSimAlt

theories/Eq/SSimAlt.v
@@ -27,6 +27,27 @@ Set Implicit Arguments.
 Arguments trans : simpl never.
 
 Section StrongSimAlt.
+  Definition ss'_gen {E F C D : Type -> Type} {X Y : Type}
+    `{HasStuck : B0 -< C} `{HasStuck' : B0 -< D}
+    (L : rel (@label E) (@label F))
+    (R Reps : rel (ctree E C X) (ctree F D Y))
+    (t : ctree E C X) (u : ctree F D Y) :=
+    (productive t -> forall l t', trans l t t' -> exists l' u', trans l' u u' /\ R t' u' /\ L l l') /\
+    (forall {Z} (c : C Z) k, t ≅ BrD c k -> forall x, exists u', epsilon u u' /\ Reps (k x) u').
+
+  Lemma ss'_gen_mon {E F C D : Type -> Type} {X Y : Type}
+    `{HasStuck : B0 -< C} `{HasStuck' : B0 -< D}
+    (L : rel (@label E) (@label F)) :
+    Proper (leq ==> leq ==> leq) (@ss'_gen E F C D X Y _ _ L).
+  Proof.
+    cbn. intros.
+    split.
+    - intros.
+      edestruct (proj1 H1) as (? & ? & ? & ?); eauto.
+      eexists _, x2; intuition; eauto.
+    - intros. edestruct (proj2 H1) as (? & ? & ?); eauto.
+  Qed.
+
 (*|
 An alternative definition [ss'] of strong simulation.
 The simulation challenge does not involve an inductive transition relation,
@@ -37,15 +58,12 @@ thus simplifying proofs.
     (L : rel (@label E) (@label F)) :
     mon (ctree E C X -> ctree F D Y -> Prop) :=
     {| body R t u :=
-      (productive t -> forall l t', trans l t t' -> exists l' u' u'', trans l' u u' /\ epsilon u' u'' /\ R t' u'' /\ L l l') /\
-      (forall {Z} (c : C Z) k, t ≅ BrD c k -> forall x, exists u', epsilon u u' /\ R (k x) u')
+      ss'_gen L R R t u
     |}.
   Next Obligation.
-    split.
-    - intros.
-      edestruct H0 as (? & ? & ? & ?); eauto.
-      eexists _, x1, x2; intuition; eauto.
-    - intros. edestruct H1 as (? & ? & ?); eauto.
+    epose proof (@ss'_gen_mon E F C D X Y _ _). eapply H1.
+    3: apply H0.
+    all: auto.
   Qed.
 
 End StrongSimAlt.
@@ -63,17 +81,17 @@ Section ssim'_theory.
    Strong simulation up-to [equ] is valid
    ----------------------------------------
 |*)
-  Lemma equ_clos_sst : equ_clos <= (t (@ss' E F C D X Y _ _ L)).
+  Lemma equ_clos_sst' : equ_clos <= (t (@ss' E F C D X Y _ _ L)).
   Proof.
     apply Coinduction; cbn.
     intros R x y [x' y' x'' y'' EQ' EQ'']. split.
     - intros prod l z x'z.
       rewrite EQ' in x'z, prod.
-      destruct ((proj1 EQ'') prod _ _ x'z) as (l' & ? & ? & ? & ? & ? & ?).
-      exists l', x0, x1.
+      destruct ((proj1 EQ'') prod _ _ x'z) as (l' & ? & ? & ? & ?).
+      exists l', x0.
       split.
       + rewrite <- Equu; auto.
-      + split; auto. split; auto.
+      + split; auto.
         eapply (f_Tf (ss' L)).
         econstructor; auto; auto.
     - intros Z c k EQx' z.
@@ -87,7 +105,7 @@ Section ssim'_theory.
   #[global] Instance equ_clos_ssim'_goal : Proper (equ eq ==> equ eq ==> flip impl) (@ssim' E F C D X Y _ _ L).
   Proof.
     cbn; intros ? ? eq1 ? ? eq2 H.
-    apply (ft_t equ_clos_sst); econstructor; [eauto | | symmetry; eauto]; assumption.
+    apply (ft_t equ_clos_sst'); econstructor; [eauto | | symmetry; eauto]; assumption.
   Qed.
 
   #[global] Instance equ_clos_ssim'_ctx : Proper (equ eq ==> equ eq ==> impl) (@ssim' E F C D X Y _ _ L).
@@ -106,8 +124,8 @@ Lemma ssim'_brD_r : forall {E F C D X Y Z} `{HasB0: B0 -< C} `{HasB0': B0 -< D}
 Proof.
   intros.
   step in H. step. split; intros.
-    + apply H in H1; auto. destruct H1 as (? & ? & ? & ? & ? & ? & ?).
-      eauto 8 with trans.
+    + apply H in H1; auto. destruct H1 as (? & ? & ? & ? & ?).
+      eauto 6 with trans.
     + eapply H in H0. destruct H0 as (? & ? & ?).
       eapply EpsilonBr in H0.
       exists x1. split. 2: apply H1. apply H0.
@@ -133,7 +151,7 @@ Proof.
     do 3 red. cbn. split; intros.
     + subst. subs.
       step in H. apply H in H1. destruct H1 as (? & ? & ? & ? & ?).
-      eexists _, _, _. split; [apply H1 |]. split; [left; reflexivity |]. split; [| apply H3].
+      eexists _, _. split; [apply H1 |]. split; [| apply H3].
       now apply CH.
     + subs. apply ssim_brD_l_inv with (x := x) in H. exists t'. split; [now left |]. now apply CH.
   - revert t t' H. coinduction R CH. intros.
@@ -145,9 +163,8 @@ Proof.
     revert t' H. induction H0; intros.
     + subs. rewrite <- ctree_eta in H1, H2, H0.
       step in H0. apply (proj1 H0) in H2; auto.
-      destruct H2 as (? & ? & ? & ? & ? & ? & ?).
-      exists x, x0. split. auto. split; auto. apply CH.
-      eapply ssim'_epsilon_r; eauto.
+      destruct H2 as (? & ? & ? & ? & ?).
+      exists x, x0. split. auto. split; auto.
     + step in H. destruct H as [_ ?].
       edestruct H as (? & ? & ?); auto.
       setoid_rewrite <- ctree_eta in IHepsilon_.
@@ -232,7 +249,7 @@ Section ssim'_homogenous_theory.
   Proof.
     apply leq_t. cbn.
     intros. unfold seq in H0. subst. split; intros.
-    - eexists _, _, _. eauto.
+    - eexists _, _. eauto.
     - eexists. split; [| auto]. subs. eright. now left.
   Qed.
 
@@ -313,45 +330,20 @@ Section ssim'_heterogenous_theory.
   Notation ssbt' L := (coinduction.bt (ss' L)).
   Notation ssT' L := (coinduction.T (ss' L)).
 
-  #[global] Instance equ_ss'_goal {RR} :
-    Proper (equ eq ==> equ eq ==> flip impl) (ss' L RR).
+  #[global] Instance equ_ss'_gen_goal {R Reps} :
+    Proper (equ eq ==> equ eq ==> flip impl) (@ss'_gen E F C D X Y _ _ L R Reps).
   Proof.
     split; intros; subs.
     - destruct H1 as [? _]. apply H in H3; auto.
-      destruct H3 as (? & ? & ? & ? & ? & ? & ?). eexists _, _, _. subs. etrans.
+      destruct H3 as (? & ? & ? & ? & ?). eexists _, _. subs. etrans.
     - destruct H1 as [_ ?]. symmetry in H. eapply H1 in H. destruct H as (? & ? & ?).
       eexists. subs. etrans.
   Qed.
 
-  #[global] Instance equ_ss'_ctx {RR} :
-    Proper (equ eq ==> equ eq ==> impl) (ss' L RR).
+  #[global] Instance equ_ss'_gen_ctx {R Reps} :
+    Proper (equ eq ==> equ eq ==> impl) (@ss'_gen E F C D X Y _ _ L R Reps).
   Proof.
     do 4 red. intros. now rewrite <- H, <- H0.
-  Qed.
-
-(*|
-   Strong simulation up-to [equ] is valid
-   ----------------------------------------
-|*)
-  Lemma equ_clos_sst' : equ_clos <= sst' L.
-  Proof.
-    apply Coinduction; cbn.
-    intros R x y [x' y' x'' y'' EQ' EQ'']. split.
-    - intros prod l z x'z.
-      rewrite EQ' in x'z, prod.
-      destruct ((proj1 EQ'') prod _ _ x'z) as (l' & ? & ? & ? & ? & ? & ?).
-      exists l', x0, x1.
-      split.
-      + rewrite <- Equu; auto.
-      + split; auto. split; auto.
-        eapply (f_Tf (ss' L)).
-        econstructor; auto; auto.
-    - intros Z c k EQx' z.
-      rewrite EQ' in EQx'.
-      destruct (proj2 EQ'' _ _ _ EQx' z) as (? & ? & ?). exists x0.
-      split.
-      + now rewrite <- Equu.
-      + eapply (f_Tf (ss' L)). econstructor. 2: apply H0. all: auto.
   Qed.
 
   #[global] Instance equ_clos_sst'_goal {RR} :
@@ -414,7 +406,8 @@ Section ssim'_heterogenous_theory.
     intros. step. now apply is_stuck_ss.
      Qed.*)
 
-  Lemma ss'_stuck (R : rel _ _) (t : ctree F D Y) b : ss' L R (stuck b) t.
+  Lemma ss'_stuck R Reps :
+    forall b (u : ctree F D Y), ss'_gen L R Reps (@stuck E C X _ b) u.
   Proof.
     split; intros.
     - destruct b; inv_trans.
@@ -461,15 +454,17 @@ Ltac __eplay_ssim' :=
 Section Proof_Rules.
 
   Arguments label: clear implicits.
-  Context {E C: Type -> Type}
-          {X : Type}
-          {HasStuck: B0 -< C}.
+  Context {E F C D : Type -> Type}
+          {X Y : Type}
+          {HasStuck: B0 -< C}
+          {HasStuck': B0 -< D}
+          {L : rel (@label E) (@label F)}.
 
-  Lemma step_ss'_ret_gen {Y F D} `{HasStuck': B0 -< D}(x : X) (y : Y) (R L : rel _ _) :
+  Lemma step_ss'_ret_gen (x : X) (y : Y) (R Reps : rel _ _) :
     R stuckD stuckD ->
     (Proper (equ eq ==> equ eq ==> impl) R) ->
     L (val x) (val y) ->
-    ss' L R (Ret x : ctree E C X) (Ret y : ctree F D Y).
+    ss'_gen L R Reps (Ret x : ctree E C X) (Ret y : ctree F D Y).
   Proof.
     intros Rstuck PROP Lval. split; intros.
     2: inv_equ.
@@ -477,7 +472,7 @@ Section Proof_Rules.
     do 3 eexists; intuition; etrans. now subs.
   Qed.
 
-  Lemma step_ss'_ret {Y F D} `{HasStuck': B0 -< D} (x : X) (y : Y) (R L : rel _ _) :
+  Lemma step_ss'_ret (x : X) (y : Y) (R : rel _ _) :
     L (val x) (val y) ->
     ssbt' L R (Ret x : ctree E C X) (Ret y : ctree F D Y).
   Proof.
@@ -494,11 +489,11 @@ Section Proof_Rules.
  transition system, stepping is hence symmetric and we can just recover
  the itree-style rule.
 |*)
-  Lemma step_ss'_vis_gen {Y Z Z' F D} `{HasStuck': B0 -< D} (e : E Z) (f: F Z')
-        (k : Z -> ctree E C X) (k' : Z' -> ctree F D Y) (R L: rel _ _) :
+  Lemma step_ss'_vis_gen {Z Z'} (e : E Z) (f: F Z')
+        (k : Z -> ctree E C X) (k' : Z' -> ctree F D Y) (R Reps : rel _ _) :
     (Proper (equ eq ==> equ eq ==> impl) R) ->
     (forall x, exists y, R (k x) (k' y) /\ L (obs e x) (obs f y)) ->
-    ss' L R (Vis e k) (Vis f k').
+    ss'_gen L R Reps (Vis e k) (Vis f k').
   Proof.
     intros. split; intros; inv_equ.
     cbn; inv_trans; subst;
@@ -508,8 +503,8 @@ Section Proof_Rules.
     - assumption.
   Qed.
 
-  Lemma step_ss'_vis {Y Z Z' F D} `{HasStuck': B0 -< D} (e : E Z) (f: F Z')
-        (k : Z -> ctree E C X) (k' : Z' -> ctree F D Y) (R L : rel _ _) :
+  Lemma step_ss'_vis {Z Z'} (e : E Z) (f: F Z')
+        (k : Z -> ctree E C X) (k' : Z' -> ctree F D Y) (R : rel _ _) :
     (forall x, exists y, sst' L R (k x) (k' y) /\ L (obs e x) (obs f y)) ->
     ssbt' L R (Vis e k) (Vis f k').
   Proof.
@@ -518,18 +513,18 @@ Section Proof_Rules.
     typeclasses eauto.
   Qed.
 
-  Lemma step_ss'_vis_id_gen {Y Z F D} `{HasStuck': B0 -< D} (e : E Z) (f: F Z)
-        (k : Z -> ctree E C X) (k' : Z -> ctree F D Y) (R L: rel _ _) :
+  Lemma step_ss'_vis_id_gen {Z} (e : E Z) (f: F Z)
+        (k : Z -> ctree E C X) (k' : Z -> ctree F D Y) (R Reps : rel _ _) :
     (Proper (equ eq ==> equ eq ==> impl) R) ->
     (forall x, R (k x) (k' x) /\ L (obs e x) (obs f x)) ->
-    ss' L R (Vis e k) (Vis f k').
+    ss'_gen L R Reps (Vis e k) (Vis f k').
   Proof.
     intros. apply step_ss'_vis_gen. { typeclasses eauto. }
     eauto.
   Qed.
 
-  Lemma step_ss'_vis_id {Y Z F D} `{HasStuck': B0 -< D} (e : E Z) (f: F Z)
-        (k : Z -> ctree E C X) (k' : Z -> ctree F D Y) (R L : rel _ _) :
+  Lemma step_ss'_vis_id {Z} (e : E Z) (f: F Z)
+        (k : Z -> ctree E C X) (k' : Z -> ctree F D Y) (R : rel _ _) :
     (forall x, sst' L R (k x) (k' x) /\ L (obs e x) (obs f x)) ->
     ssbt' L R (Vis e k) (Vis f k').
   Proof.
@@ -538,33 +533,33 @@ Section Proof_Rules.
     typeclasses eauto.
   Qed.
 
-  Lemma step_ss'_vis_l {F D Y Z L R} `{HasB0 : B0 -< C} `{HasB0' : B0 -< D} :
+  Lemma step_ss'_vis_l {Z R} :
     forall (e : E Z) (k : Z -> ctree E C X) (u : ctree F D Y),
     (forall x, exists l' u', trans l' u u' /\ t (ss' L) R (k x) u' /\ L (obs e x) l') ->
     ssbt' L R (Vis e k) u.
   Proof.
     intros. split; intros; [| inv_equ].
     inv_trans. subst. destruct (H x) as (? & ? & ? & ? & ?).
-    eexists _, _, _. rewrite <- EQ in H2. etrans.
+    eexists _, _. rewrite <- EQ in H2. etrans.
   Qed.
 
   (*|
     Same goes for visible tau nodes.
     |*)
-  Lemma step_ss'_step_gen {Y F D} `{HasTau: B1 -< C} `{HasStuck': B0 -< D} `{HasTau': B1 -< D}
-        (t : ctree E C X) (t': ctree F D Y) (R L: rel _ _):
+  Lemma step_ss'_step_gen `{HasTau: B1 -< C} `{HasTau': B1 -< D}
+        (t : ctree E C X) (t': ctree F D Y) (R Reps : rel _ _) :
     (Proper (equ eq ==> equ eq ==> impl) R) ->
     L tau tau ->
     (R t t') ->
-    ss' L R (Step t) (Step t').
+    ss'_gen L R Reps (Step t) (Step t').
   Proof.
     split; intros; inv_equ.
     inv_trans; subst.
     cbn; do 3 eexists; intuition; subs; eauto.
   Qed.
 
-  Lemma step_ss'_step {Y F D} `{HasStuck': B0 -< D} `{HasTau: B1 -< C} `{HasTau': B1 -< D}
-        (t: ctree E C X) (t': ctree F D Y) (R L : rel _ _) :
+  Lemma step_ss'_step `{HasTau: B1 -< C} `{HasTau': B1 -< D}
+        (t: ctree E C X) (t': ctree F D Y) (R : rel _ _) :
     (sst' L R t t') ->
     L tau tau ->
     ssbt' L R (Step t) (Step t').
@@ -579,20 +574,20 @@ Section Proof_Rules.
     A useful special case is the one where the arity coincide and we simply use the identity
     in both directions. We can in this case have [n] rather than [2n] obligations.
     |*)
-  Lemma step_ss'_brS_gen {Z Z' Y F D} `{HasStuck': B0 -< D} (c : C Z) (d : D Z')
-        (k : Z -> ctree E C X) (k' : Z' -> ctree F D Y) (R L: rel _ _) :
+  Lemma step_ss'_brS_gen {Z Z'} (c : C Z) (d : D Z')
+        (k : Z -> ctree E C X) (k' : Z' -> ctree F D Y) (R Reps : rel _ _) :
     (Proper (equ eq ==> equ eq ==> impl) R) ->
     (forall x, exists y, R (k x) (k' y)) ->
     L tau tau ->
-    ss' L R (BrS c k) (BrS d k').
+    ss'_gen L R Reps (BrS c k) (BrS d k').
   Proof.
     split; intros; inv_equ. inv_trans. subst.
     destruct (H0 x) as [y HR].
     cbn; do 3 eexists; intuition; subs; eauto.
   Qed.
 
-  Lemma step_ss'_brS {Z Z' Y F D} `{HasStuck' : B0 -< D} (c : C Z) (c' : D Z')
-        (k : Z -> ctree E C X) (k' : Z' -> ctree F D Y) (R L: rel _ _) :
+  Lemma step_ss'_brS {Z Z'} (c : C Z) (c' : D Z')
+        (k : Z -> ctree E C X) (k' : Z' -> ctree F D Y) (R : rel _ _) :
     (forall x, exists y, sst' L R (k x) (k' y)) ->
     L tau tau ->
     ssbt' L R (BrS c k) (BrS c' k').
@@ -602,19 +597,19 @@ Section Proof_Rules.
     typeclasses eauto.
   Qed.
 
-  Lemma step_ss'_brS_id_gen {Z Y D F} `{HasStuck': B0 -< D} (c : C Z) (d: D Z)
-        (k: Z -> ctree E C X) (k': Z -> ctree F D Y) (R L : rel _ _) :
+  Lemma step_ss'_brS_id_gen {Z} (c : C Z) (d: D Z)
+        (k: Z -> ctree E C X) (k': Z -> ctree F D Y) (R Reps : rel _ _) :
     (Proper (equ eq ==> equ eq ==> impl) R) ->
-    (forall x, exists y, R (k x) (k' y)) ->
+    (forall x, R (k x) (k' x)) ->
     L tau tau ->
-    ss' L R (BrS c k) (BrS d k').
+    ss'_gen L R Reps (BrS c k) (BrS d k').
   Proof.
     intros; apply step_ss'_brS_gen; eauto.
   Qed.
 
-  Lemma step_ss'_brS_id {Z Y D F} `{HasStuck': B0 -< D} (c : C Z) (d : D Z)
-        (k: Z -> ctree E C X) (k': Z -> ctree F D Y) (R L : rel _ _) :
-    (forall x, exists y, sst' L R (k x) (k' y)) ->
+  Lemma step_ss'_brS_id {Z} (c : C Z) (d : D Z)
+        (k: Z -> ctree E C X) (k': Z -> ctree F D Y) (R : rel _ _) :
+    (forall x, sst' L R (k x) (k' x)) ->
     L tau tau ->
     ssbt' L R (BrS c k) (BrS d k').
   Proof.
@@ -623,59 +618,59 @@ Section Proof_Rules.
     typeclasses eauto.
   Qed.
 
-  Lemma step_ss'_brS_l {F D Y Z L R} `{HasB0 : B0 -< C} `{HasB0' : B0 -< D} :
+  Lemma step_ss'_brS_l {Z R} :
     forall (c : C Z) (k : Z -> ctree E C X) (u : ctree F D Y),
     (forall x, exists l' u', trans l' u u' /\ sst' L R (k x) u' /\ L tau l') ->
          ssbt' L R (BrS c k) u.
   Proof.
     intros. split; intros; [| inv_equ].
     inv_trans. subst. destruct (H x) as (? & ? & ? & ? & ?).
-    eexists _, _, _. rewrite <- EQ in H2. etrans.
+    eexists _, _. rewrite <- EQ in H2. etrans.
   Qed.
 
   (*|
     With this definition [ss'] of simulation, delayed nodes allow to perform a coinductive step.
     |*)
-  Lemma step_ss'_brD_l_gen {Y F D Z} `{HasStuck': B0 -< D} (c : C Z)
-        (k : Z -> ctree E C X) (t': ctree F D Y) (R L: rel _ _):
-    (Proper (equ eq ==> equ eq ==> impl) R) ->
-    (forall x, R (k x) t') ->
-    ss' L R (BrD c k) t'.
+  Lemma step_ss'_brD_l_gen {Z} (c : C Z)
+        (k : Z -> ctree E C X) (t': ctree F D Y) (R Reps : rel _ _):
+    (Proper (equ eq ==> equ eq ==> impl) Reps) ->
+    (forall x, Reps (k x) t') ->
+    ss'_gen L R Reps (BrD c k) t'.
   Proof.
     split; intros. { now apply productive_brD in H1. }
     inv_equ. setoid_rewrite EQ in H0. eauto.
   Qed.
 
-  Lemma step_ss'_brD_l {Y F D Z} `{HasStuck': B0 -< D} (c : C Z)
-        (k : Z -> ctree E C X) (t: ctree F D Y) (R L: rel _ _):
+  Lemma step_ss'_brD_l {Z} (c : C Z)
+        (k : Z -> ctree E C X) (t: ctree F D Y) (R : rel _ _):
     (forall x, sst' L R (k x) t) ->
     ssbt' L R (BrD c k) t.
   Proof.
     apply step_ss'_brD_l_gen. typeclasses eauto.
   Qed.
 
-  Lemma step_ss'_brD_r_gen {Y F D Z} `{HasStuck': B0 -< D} (c : D Z) x
-        (k : Z -> ctree F D Y) (t: ctree E C X) (R L: rel _ _):
-    ss' L R t (k x) ->
-    ss' L R t (BrD c k).
+  Lemma step_ss'_brD_r_gen {Z} (c : D Z) x
+        (k : Z -> ctree F D Y) (t: ctree E C X) (R Reps : rel _ _):
+    ss'_gen L R Reps t (k x) ->
+    ss'_gen L R Reps t (BrD c k).
   Proof.
     cbn. split; intros.
-    apply H in H1 as (? & ? & ? & ? & ? & ? & ?).
-    exists x0, x1, x2; etrans. auto.
+    apply H in H1 as (? & ? & ? & ? & ?).
+    exists x0, x1; etrans. auto.
     eapply (proj2 H) in H0 as (? & ? & ?). eapply EpsilonBr in H0. etrans.
   Qed.
 
-  Lemma step_ss'_brD_r {Y F D Z} `{HasStuck': B0 -< D} (c : D Z) x
-        (k : Z -> ctree F D Y) (t: ctree E C X) (R L: rel _ _):
+  Lemma step_ss'_brD_r {Z} (c : D Z) x
+        (k : Z -> ctree F D Y) (t: ctree E C X) (R : rel _ _):
     ssbt' L R t (k x) ->
     ssbt' L R t (BrD c k).
   Proof.
     intros. eapply step_ss'_brD_r_gen. apply H.
   Qed.
 
-  Lemma step_ss'_epsilon_r_gen : forall {F D Y} `{HasB0': B0 -< D}
-    L (t : ctree E C X) (u u' : ctree F D Y) (R : rel _ _),
-    ss' L R t u' -> epsilon u u' -> ss' L R t u.
+  Lemma step_ss'_epsilon_r_gen :
+    forall (t : ctree E C X) (u u' : ctree F D Y) (R Reps : rel _ _),
+    ss'_gen L R Reps t u' -> epsilon u u' -> ss'_gen L R Reps t u.
   Proof.
     intros. red in H0. rewrite (ctree_eta u). rewrite (ctree_eta u') in H.
     genobs u ou. genobs u' ou'. clear u Heqou u' Heqou'.
@@ -685,78 +680,78 @@ Section Proof_Rules.
       eapply step_ss'_brD_r_gen. apply H.
   Qed.
 
-  Lemma step_ss'_epsilon_r : forall {F D Y} `{HasB0': B0 -< D}
-    L (t : ctree E C X) (u u' : ctree F D Y) (R : rel _ _),
+  Lemma step_ss'_epsilon_r :
+    forall (t : ctree E C X) (u u' : ctree F D Y) (R : rel _ _),
     ssbt' L R t u' -> epsilon u u' -> ssbt' L R t u.
   Proof.
     intros. eapply step_ss'_epsilon_r_gen. apply H. apply H0.
   Qed.
 
-  Lemma step_ss'_brD_gen {Y F D n m} `{HasStuck': B0 -< D} (a: C n) (b: D m)
-    (k : n -> ctree E C X) (k' : m -> ctree F D Y) (R L : rel _ _) :
-    (Proper (equ eq ==> equ eq ==> impl) R) ->
-    (forall x, exists y, R (k x) (k' y)) ->
-    ss' L R (BrD a k) (BrD b k').
+  Lemma step_ss'_brD_gen {Z Z'} (a: C Z) (b: D Z')
+    (k : Z -> ctree E C X) (k' : Z' -> ctree F D Y) (R Reps : rel _ _) :
+    (Proper (equ eq ==> equ eq ==> impl) Reps) ->
+    (forall x, exists y, Reps (k x) (k' y)) ->
+    ss'_gen L R Reps (BrD a k) (BrD b k').
   Proof.
     split; intros. { now apply productive_brD in H1. }
     inv_equ. setoid_rewrite EQ in H0. destruct (H0 x).
     eexists. split; [| eassumption]. eright. eleft. reflexivity.
   Qed.
 
-  Lemma step_ss'_brD {Y F D n m} `{HasStuck': B0 -< D} (cn: C n) (cm: D m)
-    (k : n -> ctree E C X) (k' : m -> ctree F D Y) (L R : rel _ _) :
+  Lemma step_ss'_brD {Z Z'} (cn: C Z) (cm: D Z')
+    (k : Z -> ctree E C X) (k' : Z' -> ctree F D Y) (R : rel _ _) :
     (forall x, exists y, sst' L R (k x) (k' y)) ->
     ssbt' L R (BrD cn k) (BrD cm k').
   Proof.
     apply step_ss'_brD_gen. typeclasses eauto.
   Qed.
 
-  Lemma step_ss'_brD_id_gen {F D Y Z} `{HasStuck': B0 -< D} (c: C Z) (d: D Z)
+  Lemma step_ss'_brD_id_gen {Z} (c: C Z) (d: D Z)
         (k : Z -> ctree E C X) (k' : Z -> ctree F D Y)
-        (R L : rel _ _) :
-    (Proper (equ eq ==> equ eq ==> impl) R) ->
-    (forall x, R (k x) (k' x)) ->
-    ss' L R (BrD c k) (BrD d k').
+        (R Reps : rel _ _) :
+    (Proper (equ eq ==> equ eq ==> impl) Reps) ->
+    (forall x, Reps (k x) (k' x)) ->
+    ss'_gen L R Reps (BrD c k) (BrD d k').
   Proof.
    intros. apply step_ss'_brD_gen; eauto.
   Qed.
 
-  Lemma step_ss'_brD_id {F D Y Z} `{HasStuck': B0 -< D} (c: C Z) (d: D Z)
-    (k : Z -> ctree E C X) (k': Z -> ctree F D Y) (R L: rel _ _) :
+  Lemma step_ss'_brD_id {Z} (c: C Z) (d: D Z)
+    (k : Z -> ctree E C X) (k': Z -> ctree F D Y) (R : rel _ _) :
     (forall x, sst' L R (k x) (k' x)) ->
     ssbt' L R (BrD c k) (BrD d k').
   Proof.
     apply step_ss'_brD_id_gen. typeclasses eauto.
   Qed.
 
-  Lemma step_ss'_guard_l_gen {Y F D} `{HasStuck': B0 -< D} `{HasTau: B1 -< C} `{HasTau': B1 -< D}
-        (t: ctree E C X) (t': ctree F D Y) (R L: rel _ _):
-    (Proper (equ eq ==> equ eq ==> impl) R) ->
-    R t t' ->
-    ss' L R (Guard t) t'.
+  Lemma step_ss'_guard_l_gen `{HasTau: B1 -< C} `{HasTau': B1 -< D}
+        (t: ctree E C X) (t': ctree F D Y) (R Reps : rel _ _):
+    (Proper (equ eq ==> equ eq ==> impl) Reps) ->
+    Reps t t' ->
+    ss'_gen L R Reps (Guard t) t'.
   Proof.
     intros. apply step_ss'_brD_l_gen; auto.
   Qed.
 
-  Lemma step_ss'_guard_l {Y F D} `{HasStuck': B0 -< D} `{HasTau: B1 -< C} `{HasTau': B1 -< D}
-        (t: ctree E C X) (t': ctree F D Y) (R L: rel _ _):
+  Lemma step_ss'_guard_l `{HasTau: B1 -< C} `{HasTau': B1 -< D}
+        (t: ctree E C X) (t': ctree F D Y) (R : rel _ _):
     sst' L R t t' ->
     ssbt' L R (Guard t) t'.
   Proof.
     apply step_ss'_guard_l_gen. typeclasses eauto.
   Qed.
 
-  Lemma step_ss'_guard_gen {Y F D} `{HasStuck': B0 -< D} `{HasTau: B1 -< C} `{HasTau': B1 -< D}
-        (t: ctree E C X) (t': ctree F D Y) (R L: rel _ _):
-    (Proper (equ eq ==> equ eq ==> impl) R) ->
-    R t t' ->
-    ss' L R (Guard t) (Guard t').
+  Lemma step_ss'_guard_gen `{HasTau: B1 -< C} `{HasTau': B1 -< D}
+        (t: ctree E C X) (t': ctree F D Y) (R Reps : rel _ _):
+    (Proper (equ eq ==> equ eq ==> impl) Reps) ->
+    Reps t t' ->
+    ss'_gen L R Reps (Guard t) (Guard t').
   Proof.
     intros. apply step_ss'_brD_id_gen; auto.
   Qed.
 
-  Lemma step_ss'_guard {Y F D} `{HasStuck': B0 -< D} `{HasTau: B1 -< C} `{HasTau': B1 -< D}
-        (t: ctree E C X) (t': ctree F D Y) (R L: rel _ _):
+  Lemma step_ss'_guard `{HasTau: B1 -< C} `{HasTau': B1 -< D}
+        (t: ctree E C X) (t': ctree F D Y) (R : rel _ _):
     sst' L R t t' ->
     ssbt' L R (Guard t) (Guard t').
   Proof.
@@ -782,21 +777,10 @@ Section bind.
           (L : hrel (@label E) (@label F)) (R0 : rel X Y).
 
 (*|
-Specialization of [bind_ctx] to a function acting with [ssim] on the bound value,
-and with the argument (pointwise) on the continuation.
-|*)
-  Program Definition bind_ctx_ssim' L0 : mon (rel (ctree E C X') (ctree F D Y')) :=
-    {|body := fun R => @bind_ctx E F C D X Y X' Y' (ssim' L0) (pointwise R0 R) |}.
-  Next Obligation.
-    intros ?? ? H. apply leq_bind_ctx. intros ?? H' ?? H''.
-    apply in_bind_ctx. apply H'. intros t t' HS. apply H, H'', HS.
-  Qed.
-
-(*|
     The resulting enhancing function gives a valid up-to technique
 |*)
   Lemma bind_ctx_ssim'_t L0 (*{RV: Respects_val L}*):
-    is_update_val_rel L R0 L0 -> bind_ctx_ssim' L0 <= (t (ss' L)).
+    is_update_val_rel L R0 L0 -> @bind_ctx_ssim E F C D X X' Y Y' _ _ R0 L0 <= (t (ss' L)).
   Proof.
     intro HL0. apply Coinduction.
     intros R. apply (leq_bind_ctx _).
@@ -804,51 +788,41 @@ and with the argument (pointwise) on the continuation.
     step in tt. split.
     - simpl; intros PROD l u STEP.
       apply trans_bind_inv in STEP as [(H & t' & STEP & EQ) | (v & STEPres & STEP)].
-      apply tt in STEP as (l' & u' & u'' & STEP & EPS & EQ' & ?).
-      2: { now apply productive_bind in PROD. }
-      do 3 eexists. split; [| split; [| split]].
+      apply tt in STEP as (l' & u' & STEP & EQ' & ?).
+      do 2 eexists. split; [| split].
       apply trans_bind_l; eauto.
       + intro Hl. destruct Hl.
-        apply HL0 in H0.
-        2: now apply wf_val_nonval.
-        2: now apply wf_val_trans in STEP.
+        apply HL0 in H0; etrans.
         inversion H0; subst. apply H. constructor. apply H2. constructor.
-      + apply epsilon_bind_l. apply EPS.
       + apply (fT_T equ_clos_sst').
-          econstructor; [exact EQ | | reflexivity].
-          apply (fTf_Tf (ss' L)).
-          apply in_bind_ctx; [apply EQ' |].
-          intros ? ? ?.
-          apply (b_T (ss' L)).
-          red in kk; cbn; apply kk. eassumption.
-      + apply HL0 in H0.
-        2: now apply wf_val_nonval.
-        2: now apply wf_val_trans in STEP.
+        econstructor; [exact EQ | | reflexivity].
+        apply (fTf_Tf (ss' L)).
+        apply in_bind_ctx; [apply EQ' |].
+        intros ? ? ?.
+        apply (b_T (ss' L)).
+        red in kk; cbn; apply kk. eassumption.
+      + apply HL0 in H0; etrans.
         destruct H0. exfalso. apply H. constructor. apply H2.
       + assert (t1 ≅ Ret v).
         { apply productive_bind in PROD. apply trans_val_epsilon in STEPres as [? _].
           now apply productive_epsilon. } subs.
-        apply tt in STEPres as (l' & u' & u'' & STEPres & EPS & EQ' & ?).
-        2: { now apply productive_bind in PROD. }
-        apply HL0 in H.
-        2: apply wf_val_val.
-        2: now apply wf_val_trans in STEPres.
+        apply tt in STEPres as (l' & u' & STEPres & EQ' & ?).
+        apply HL0 in H; etrans.
         dependent destruction H. 2: { exfalso. apply H. constructor. }
         pose proof (trans_val_inv STEPres) as EQ.
         rewrite EQ in STEPres.
         specialize (kk v v2 H).
         rewrite bind_ret_l in PROD.
-        apply kk in STEP as (? & u''' & ? & STEP & EPS' & EQ'' & ?); auto.
-        do 3 eexists; split.
+        apply kk in STEP as (? & u''' & STEP & EQ'' & ?); auto.
+        do 2 eexists; split.
         eapply trans_bind_r; eauto.
-        split; [eassumption |]. split; auto.
+        split; auto.
         eapply (id_T (ss' L)); auto.
     - intros Z c k EQ z.
       apply br_equ_bind in EQ as EQ'. destruct EQ' as [(v & EQ') | (k0 & EQ' & EQ'')].
-      + subs. destruct tt as [tt _].
-        edestruct tt as (l & t'' & _ & STEPres & _ & _ & ?).
-        now eapply prod_ret. etrans.
-        apply HL0 in H. 2: apply wf_val_val. 2: now apply wf_val_trans in STEPres.
+      + subs.
+        edestruct tt as (l & t'' & STEPres & _ & ?). etrans.
+        apply HL0 in H; etrans.
         apply update_val_rel_val_l in H as (v' & -> & EQ').
         rewrite bind_ret_l in EQ.
         specialize (kk v v' EQ'). apply kk with (x := z) in EQ. destruct EQ as (u' & EPS & EQ).
@@ -856,14 +830,11 @@ and with the argument (pointwise) on the continuation.
         apply trans_val_epsilon in STEPres as [? _]. split.
         * eapply epsilon_bind; eassumption.
         * now apply (id_T (ss' L)).
-      + subs. destruct tt as [_ tt].
-        specialize (tt Z c k0). lapply tt; [clear tt; intros tt | reflexivity].
-        destruct (tt z) as (u' & EPS & tt').
-        exists (u' >>= k2). split.
-        * now apply epsilon_bind_l.
-        * rewrite EQ''.
-          apply (fTf_Tf (ss' L)). apply in_bind_ctx. apply tt'.
-          red. intros. apply (b_T (ss' L)). now apply kk.
+      + subs. eexists. split; [now left |].
+        rewrite EQ''.
+        apply (fTf_Tf (ss' L)). apply in_bind_ctx.
+        eapply ssim_brD_l_inv. step. apply tt.
+        red. intros. apply (b_T (ss' L)). now apply kk.
   Qed.
 
 End bind.
@@ -877,12 +848,27 @@ Lemma sst'_clo_bind {E F C D: Type -> Type} {X Y X' Y': Type} {L : rel (@label E
       (t1 : ctree E C X) (t2: ctree F D Y)
       (HL0 : is_update_val_rel L R0 L0)
       (k1 : X -> ctree E C X') (k2 : Y -> ctree F D Y') RR:
-  ssim' L0 t1 t2 ->
+  ssim L0 t1 t2 ->
   (forall x y, R0 x y -> (sst' L RR) (k1 x) (k2 y)) ->
   sst' L RR (t1 >>= k1) (t2 >>= k2).
 Proof.
   intros ? ?.
   apply (ft_t (@bind_ctx_ssim'_t E F C D X X' Y Y' _ _ L R0 L0 HL0)).
+  apply in_bind_ctx; eauto.
+Qed.
+
+Lemma ssbt'_clo_bind {E F C D: Type -> Type} {X Y X' Y': Type} {L : rel (@label E) (@label F)}
+      `{HasStuck: B0 -< C} `{HasStuck': B0 -< D}
+      (R0 : rel X Y) L0
+      (t1 : ctree E C X) (t2: ctree F D Y)
+      (HL0 : is_update_val_rel L R0 L0)
+      (k1 : X -> ctree E C X') (k2 : Y -> ctree F D Y') RR:
+  ssim L0 t1 t2 ->
+  (forall x y, R0 x y -> (ssbt' L RR) (k1 x) (k2 y)) ->
+  ssbt' L RR (t1 >>= k1) (t2 >>= k2).
+Proof.
+  intros ? ?.
+  apply (fbt_bt (@bind_ctx_ssim'_t E F C D X X' Y Y' _ _ L R0 L0 HL0)).
   apply in_bind_ctx; eauto.
 Qed.
 
